Add bind to tau spec + related lemmas

iodiv/DivFreeTauSpec.fst
@@ -145,6 +145,12 @@ let iwp_monotonic #a (w : iwp' a) =
 let iwp a =
   w : iwp' a { iwp_monotonic w }
 
+let iwp_monotonic_inst #a (w : iwp a) p q hist :
+  Lemma
+    (requires w p hist /\ p `i_post_le` q)
+    (ensures w q hist)
+= ()
+
 let ile #a (w w' : iwp a) =
   forall p. w' p `i_pre_le` w p
 
@@ -195,6 +201,143 @@ let ishift_post_nil #a (post : i_post a) :
     match r with
     | Ocv tr x -> ()
     | Odv s -> stream_prepend_nil s ; stream_ext (stream_prepend [] s) s
+  end
+
+let ishift_post_mono a tr :
+  Lemma (forall (p q : i_post a). p `i_post_le` q ==> ishift_post tr p `i_post_le` ishift_post tr q)
+= ()
+
+let ishift_post_app #a t t' (p : i_post a) :
+  Lemma (ishift_post (t' @ t) p `i_post_le` ishift_post t (ishift_post t' p))
+= introduce forall r. ishift_post (t' @ t) p r ==> ishift_post t (ishift_post t' p) r
+  with begin
+    match r with
+    | Ocv tr x -> append_assoc t' t tr
+    | Odv st -> stream_prepend_app t' t st
+  end
+
+let i_bind_post' #a #b (wf : a -> iwp b) (post : i_post b) hist : i_post' a =
+  fun r ->
+    match r with
+    | Ocv tr x -> wf x (ishift_post tr post) (rev_acc (to_trace tr) hist)
+    | Odv st -> post (Odv st)
+
+let i_bind_post #a #b (wf : a -> iwp b) (post : i_post b) hist : i_post a =
+  introduce forall r r'. r `eutt` r' /\ i_bind_post' wf post hist r ==> i_bind_post' wf post hist r'
+  with begin
+    introduce r `eutt` r' /\ i_bind_post' wf post hist r ==> i_bind_post' wf post hist r'
+    with _. begin
+      match r, r' with
+      | Ocv t x, Ocv t' x' ->
+        introduce forall r. ishift_post t post r ==> ishift_post t' post r
+        with begin
+          introduce ishift_post t post r ==> ishift_post t' post r
+          with _. begin
+            match r with
+            | Ocv tr y ->
+              to_trace_append t tr ;
+              to_trace_append t' tr ;
+              assert (Ocv (t @ tr) y `eutt` Ocv (t' @ tr) y) ;
+              i_post_resp_eutt post (Ocv (t @ tr) y) (Ocv (t' @ tr) y)
+            | Odv s ->
+              uptotau_prepend t t' s s ;
+              assert (Odv (stream_prepend t s) `eutt #a` Odv (stream_prepend t' s)) ;
+              i_post_resp_eutt post (Odv (stream_prepend t s)) (Odv (stream_prepend t' s))
+          end
+        end ;
+        iwp_monotonic_inst (wf x) (ishift_post t post) (ishift_post t' post) (rev_acc (to_trace t) hist)
+      | Odv s, Odv s' ->
+        i_post_resp_eutt post (Odv s) (Odv s')
+    end
+  end ;
+  i_bind_post' wf post hist
+
+let i_bind_post_mono #a #b (wf : a -> iwp b) p q hist :
+  Lemma
+    (requires p `i_post_le` q)
+    (ensures i_bind_post wf p hist `i_post_le` i_bind_post wf q hist)
+= introduce forall r. i_bind_post wf p hist r ==> i_bind_post wf q hist r
+  with begin
+    match r with
+    | Ocv tr x ->
+      ishift_post_mono b tr ;
+      assert (ishift_post tr p `i_post_le` ishift_post tr q) ;
+      assert (wf x (ishift_post tr p) (rev_acc (to_trace tr) hist) ==> wf x (ishift_post tr q) (rev_acc (to_trace tr) hist))
+    | Odv s -> ()
+  end
+
+let i_bind (#a : Type u#a) (#b : Type u#b) (w : iwp a) (wf : a -> iwp b) : iwp b =
+  introduce forall p q hist. p `i_post_le` q ==> i_bind_post wf p hist `i_post_le` i_bind_post wf q hist
+  with begin
+    move_requires (i_bind_post_mono wf p q) hist
+  end ;
+  as_iwp (fun post hist ->
+    w (i_bind_post wf post hist) hist
+  )
+
+let i_bind_mono #a #b (w : iwp a) (wf wf' : a -> iwp b) :
+  Lemma
+    (requires forall x. wf x `ile` wf' x)
+    (ensures i_bind w wf `ile` i_bind w wf')
+= introduce forall post hist. i_bind w wf' post hist ==> i_bind w wf post hist
+  with begin
+    assert (i_bind_post wf' post hist `i_post_le` i_bind_post wf post hist)
+  end
+
+let i_bind_cong #a #b (w : iwp a) (wf wf' : a -> iwp b) :
+  Lemma
+    (requires forall x. wf x `ieq` wf' x)
+    (ensures i_bind w wf `ieq` i_bind w wf')
+= i_bind_mono w wf wf' ;
+  i_bind_mono w wf' wf
+
+let i_bind_assoc #a #b #c (w : iwp a) (wf : a -> iwp b) (wg : b -> iwp c) :
+  Lemma (i_bind w (fun x -> i_bind (wf x) wg) `ile` i_bind (i_bind w wf) wg)
+= introduce forall post hist. i_bind (i_bind w wf) wg post hist ==> i_bind w (fun x -> i_bind (wf x) wg) post hist
+  with begin
+    introduce forall r. i_bind_post wf (i_bind_post wg post hist) hist r ==> i_bind_post (fun x -> i_bind (wf x) wg) post hist r
+    with begin
+      match r with
+      | Ocv tr x ->
+        introduce forall r'. ishift_post tr (i_bind_post wg post hist) r' ==> i_bind_post wg (ishift_post tr post) (rev_acc (to_trace tr) hist) r'
+        with begin
+          match r' with
+          | Ocv tr' y ->
+            to_trace_append tr tr' ;
+            rev_acc_rev' (to_trace tr @ to_trace tr') hist ; // rev_acc (to_trace tr @ to_trace tr') hist == rev' (to_trace tr @ to_trace tr') @ hist
+            rev'_append (to_trace tr) (to_trace tr') ; // == (rev' (to_trace tr') @ rev' (to_trace tr)) @ hist
+            append_assoc (rev' (to_trace tr')) (rev' (to_trace tr)) hist ; // == rev' (to_trace tr') @ rev' (to_trace tr) @ hist
+            rev_acc_rev' (to_trace tr) hist ; // == rev' (to_trace tr') @ rev_acc (to_trace tr) hist
+            rev_acc_rev' (to_trace tr') (rev_acc (to_trace tr) hist) ; // == rev_acc (to_trace tr') (rev_acc (to_trace tr) hist)
+            ishift_post_app tr' tr post
+          | Odv st -> ()
+        end ;
+        assert (ishift_post tr (i_bind_post wg post hist) `i_post_le` i_bind_post wg (ishift_post tr post) (rev_acc (to_trace tr) hist))
+      | Odv st -> ()
+    end ;
+    assert (i_bind_post wf (i_bind_post wg post hist) hist `i_post_le` i_bind_post (fun x -> i_bind (wf x) wg) post hist)
+  end
+
+let i_bind_post_ret #a (post : i_post a) hist :
+  Lemma (i_bind_post i_ret post hist `i_post_eq` post)
+= introduce forall r. i_bind_post i_ret post hist r <==> post r
+  with begin
+    match r with
+    | Ocv tr x -> ()
+    | Odv st -> ()
+  end
+
+let i_bind_ret #a (w : iwp a) :
+  Lemma (i_bind w i_ret `ieq` w)
+= introduce forall post hist. i_bind w i_ret post hist <==> w post hist
+  with begin
+    calc (<==>) {
+      i_bind w i_ret post hist ;
+      == {}
+      w (i_bind_post i_ret post hist) hist ;
+      <==> { i_bind_post_ret post hist }
+      w post hist ;
+    }
   end
 
 // TODO
